stdlib/boxed/extra_specs.v
@@ -26,10 +26,62 @@ Section contractive.
         repeat solve_proper_step.
       + solve_proper_prepare.
         repeat solve_proper_step.
-    - cbn; apply _. 
+    - cbn; apply _.
   Qed.
   Global Instance Box_inv_t_ne {rt1 T_rt A_rt : RT} (T : type rt1 → type T_rt) (A_ty : type A_rt) (A_attrs : Allocator_spec_attrs A_rt) :
     TypeNonExpansive T →
     TypeNonExpansive (λ ty, Box_inv_t T_rt A_rt A_attrs <TY> (T ty) <TY> A_ty <INST!>).
   Proof. apply _. Qed.
+
+  (** Resolve ghost: Resolve observations on the contained value. *)
+  Lemma resolve_ghost_box {T_rt A_rt} A_attrs (T_ty : type T_rt) (A_ty : type A_rt) π E L r rm T :
+    (∀ l', resolve_ghost π E L rm true l' (◁ T_ty) (Owned false) r T)
+    ⊢ resolve_ghost_adt π E L rm r (Box_inv_t T_rt A_rt A_attrs <TY> T_ty <TY> A_ty <INST!>) T.
+  Proof.
+    rewrite /resolve_ghost_adt /resolve_ghost.
+    iIntros "HT" (????) "#CTX #HE HL Hv".
+    iEval (rewrite /ty_own_val/=) in "Hv".
+    iDestruct "Hv" as ((l' & a & [])) "(Hinv & Hv)". simpl in *.
+    iDestruct "Hinv" as "(%l'' & %a'' & %Heq & Hl' & Halloc & _)".
+    inversion Heq. subst.
+    unfold guarded. iDestruct "Hl'" as "(Hc & Hl')".
+    iDestruct "Hc" as "((Hc1 & Hc) & Ht)".
+    iApply (lc_fupd_add_later with "Hc1"). iNext.
+    iMod ("HT" with "[] [] CTX HE HL Hl'") as "(%L2 & %r' & %R & %progress & Hstep & HL & HT)"; [done.. | ].
+    iFrame.
+    iApply (logical_step_compose with "Hstep").
+    iApply (logical_step_intro_tr with "Ht").
+    iModIntro. iIntros "Ht Hcreds' !> (Hl' & $)".
+    iEval (rewrite /ty_own_val/=).
+    iFrame. iR.
+    rewrite /guarded. iFrame.
+    iDestruct "Ht" as "(_ & $)".
+  Qed.
+
+  (* Box is covariant in T and A *)
+  Lemma subtype_box {T_rt A_rt} A_attrs (T_ty_1 T_ty_2 : type T_rt) (A_ty_1 A_ty_2 : type A_rt) E L T :
+    mut_subtype E L T_ty_1 T_ty_2 (mut_subtype E L A_ty_1 A_ty_2 T)
+    ⊢ subtype_adt E L (Box_inv_t_inv_spec T_rt A_rt A_attrs <TY> T_ty_1 <TY> A_ty_1 <INST!>) (Box_inv_t_inv_spec T_rt A_rt A_attrs <TY> T_ty_2 <TY> A_ty_2 <INST!>) T.
+  Proof.
+    rewrite /mut_subtype /subtype_adt.
+    iIntros "(%HsubT & %HsubA & $)". iPureIntro.
+    iIntros (?) "HL HE".
+    iPoseProof (full_subtype_acc_noend with "HE HL") as "#HinclT"; first apply HsubT.
+    iPoseProof (full_subtype_acc_noend with "HE HL") as "#HinclA"; first apply HsubA.
+    iSplit; iModIntro.
+    - iIntros (? x r). simpl.
+      iIntros "(%l & %a & -> & Hl & Hperm)".
+      iExists _, _. iR.
+      iDestruct ("HinclT" $! inhabitant) as "(%Hst & _ )".
+      rewrite Hst. iFrame.
+      iApply (guarded_mono with "[] Hl").
+      iIntros "Hl". by iApply type_incl_ltype_owned_wand.
+    - iIntros (? ? x r). simpl.
+      iIntros "(%l & %a & -> & Hl & Hperm)".
+      iExists _, _. iR. iL.
+      iApply (guarded_mono with "[] Hl").
+      iIntros "Hl". by iApply type_incl_ltype_shared_wand.
+  Qed.
+  Definition subtype_box_inst := [instance @subtype_box].
+  Global Existing Instance subtype_box_inst.
 End contractive.
